GoLean/GoCore.lean
@@ -1,2 +1,3 @@
 import GoLean.GoCore.Machine
 import GoLean.GoCore.StepFn
+import GoLean.GoCore.MachineSound
